StmtRelML.thy
@@ -129,6 +129,7 @@ ML \<open>
        exp_rel_info   (* rhs *)
   | InhaleHint of (atomic_inhale_rel_hint inhale_rel_complete_hint)
   | ExhaleHint of (atomic_exhale_rel_hint exhale_rel_complete_hint)
+  | AssertHint of (atomic_exhale_rel_hint assert_rel_complete_hint)
   | MethodCallHint of 
        string * (* callee name *)
        thm list * (* Boogie return variable lookup decl theorem *)
@@ -256,6 +257,26 @@ ML \<open>
             exhale_havoc_tac ctxt (#basic_info info) lookup_decl_exhale_heap_thm
        | NONE => exhale_pure_no_havoc_tac ctxt
     )
+
+  fun assert_rel_tac ctxt (info: 'a exhale_rel_info) (hint: 'a assert_rel_complete_hint) =
+    (Rmsg' "stmt rel assert exhale rel pre propagate" (resolve_tac ctxt @{thms exhale_rel_propagate_pre_no_inv}) ctxt) THEN'
+    (Rmsg' "stmt rel assert propagate progress" (resolve_tac ctxt @{thms red_ast_bpl_rel_transitive} THEN' (progress_red_bpl_rel_tac ctxt)) ctxt) THEN'
+(*    (Rmsg' "stmt rel assert track well-def" (resolve_tac ctxt [@{thm red_ast_bpl_rel_weaken_input} OF @{thms state_rel_def_same_to_state_rel}] THEN' assm_full_simp_solved_tac ctxt) ctxt) THEN'*)
+    (Rmsg' "stmt rel assert setup well-def state exhale" ((#setup_well_def_state_tac hint) (#basic_info info) ctxt) ctxt) THEN'
+    (Rmsg' "stmt rel assert exhale rel post propagate" (resolve_tac ctxt @{thms exhale_rel_propagate_posts_same_exh}) ctxt) THEN'
+     exhale_rel_aux_tac ctxt info (#exhale_rel_hint hint) THEN'
+    (Rmsg' "stmt rel assert exhale rel revert well-def vars" (exhale_revert_state_relation ctxt (#basic_info info)) ctxt) THEN'
+    (Rmsg' "stmt rel assert reset state" ((#reset_state_tac hint) (#basic_info info) ctxt) ctxt)
+  
+  fun assert_rel_init_tac_standard setup_assert_state_tacs (basic_info: basic_stmt_rel_info) ctxt =
+    
+    (Rmsg' "assert rel mask and heap var" (assm_full_simp_solved_with_thms_tac [#tr_def_thm basic_info] ctxt) ctxt) THEN'
+    (Rmsg' "assert rel invariant" (assm_full_simp_solved_tac ctxt) ctxt) THEN'
+    (Rmsg' "assert rel setup assert propagate" (resolve_tac ctxt @{thms exhale_rel_propagate_pre_no_inv_same_exh}) ctxt) THEN'
+    (Rmsg' "assert rel setup assert state tac" 
+              (EVERY'_red_ast_bpl_rel_transitive_with_inv_fst_eq_snd ctxt (map (fn tac => tac basic_info) setup_assert_state_tacs)) ctxt) THEN'
+    (Rmsg' "assert rel show state rel capture init 1" (resolve_tac ctxt @{thms red_ast_bpl_rel_input_implies_output}) ctxt) THEN'
+    (Rmsg' "assert rel show state rel capture init 2" (state_rel_capture_state_intro ctxt) ctxt)      
                  
   fun atomic_rel_inst_tac ctxt (inhale_info: atomic_inhale_rel_hint inhale_rel_info) (exhale_info: atomic_exhale_rel_hint exhale_rel_info) (basic_info : basic_stmt_rel_info) (atomic_hint : atomic_rel_hint)  = 
     (case atomic_hint of 
@@ -272,6 +293,10 @@ ML \<open>
         (Rmsg' "AtomicExh2 Consistency" (fastforce_tac ctxt []) ctxt) THEN'
         (Rmsg' "AtomicExh3 Invariant" (assm_full_simp_solved_tac ctxt) ctxt) THEN'
         (exhale_rel_tac ctxt exhale_info exh_complete_hint)
+     | AssertHint assert_complete_hint =>
+        (Rmsg' "AtomicAssert Start" (resolve_tac ctxt [#assert_stmt_rel_thm assert_complete_hint]) ctxt) THEN'
+        (Rmsg' "AtomicAssert Init" ((#init_tac assert_complete_hint) basic_info ctxt) ctxt) THEN'         
+        (assert_rel_tac ctxt exhale_info assert_complete_hint)
      | MethodCallHint (callee_name, rets_lookup_decl_thms, inhale_info_call, exhale_info_call, exh_pre_complete_hint, inh_post_complete_hint) => 
         let val callee_data = Symtab.lookup (#method_data_table basic_info) callee_name |> Option.valOf in
         (Rmsg' "MethodCall Start" (resolve_tac ctxt [@{thm method_call_stmt_rel} OF [#consistency_wf_thm basic_info, #consistency_down_mono_thm basic_info]]) ctxt) THEN'
